one more file

VCVio/OracleComp/QueryTracking/LoggingOracle.lean
@@ -36,7 +36,7 @@ end QueryImpl
 /-- Simulation oracle for tracking the quries in a `QueryLog`, without modifying the actual
 behavior of the oracle. Requires decidable equality of the indexing set to determine
 which list to update when queries come in. -/
-def loggingOracle (spec : OracleSpec ι) :
+def loggingOracle {spec : OracleSpec ι} :
     QueryImpl spec (WriterT (QueryLog spec) (OracleComp spec)) :=
   (QueryImpl.ofLift spec (OracleComp spec)).withLogging
 
@@ -47,7 +47,7 @@ lemma probFailure_simulateQ {spec : OracleSpec.{0,0} ι} {α : Type}
     [spec.Fintype] [spec.Inhabited]
     (oa : OracleComp spec α) :
     Pr[⊥ | (WriterT.run
-        (simulateQ (loggingOracle (spec := spec)) oa : WriterT (QueryLog spec) (OracleComp spec) α) :
+        (simulateQ (loggingOracle (spec := spec)) oa) :
           OracleComp spec (α × spec.QueryLog))] = Pr[⊥ | oa] := by
   induction oa using OracleComp.induction with
   | pure a => simp
